src/Ex/MsiSvInvB.v
@@ -1,0 +1,163 @@
+Require Import Bool List String Peano_dec Lia.
+Require Import Common FMap HVector Syntax Topology Semantics SemFacts StepM.
+Require Import Invariant TrsInv Simulation Serial SerialFacts.
+Require Import RqRsLang RqRsCorrect.
+
+Require Import Msi MsiSv SpecSv MsiSvTopo.
+
+Set Implicit Arguments.
+
+Import MonadNotations.
+Import CaseNotations.
+
+Open Scope list.
+Open Scope hvec.
+Open Scope fmap.
+
+Ltac solve_msi :=
+  unfold msiM, msiS, msiI in *; lia.
+
+Ltac solve_msi_false :=
+  exfalso; try congruence;
+  match goal with
+  | [H: msiS <= msiI |- _] => clear -H; solve_msi
+  | [H: msiM <= msiI |- _] => clear -H; solve_msi
+  | [H: msiM <= msiS |- _] => clear -H; solve_msi
+  | [H1: ?t = msiI, H2: msiS <= ?t |- _] =>
+    rewrite H1 in H2; clear -H2; solve_msi
+  | [H1: ?t = msiI, H2: msiM <= ?t |- _] =>
+    rewrite H1 in H2; clear -H2; solve_msi
+  | [H1: ?t = msiS, H2: msiM <= ?t |- _] =>
+    rewrite H1 in H2; clear -H2; solve_msi
+  end.
+
+Section Inv.
+
+  Section InvDir.
+    Variables (post: OState ImplOStateIfc)
+              (porq: ORq Msg).
+
+    (* Why soundness of the shared status:
+     * the parent is upgraded to M when all children values are evicted.
+     * In this case the parent does not update the value, but maintain the
+     * value since the protocol is write-through. But in order to check
+     * correctness we need to know the parent status is S when all children
+     * values are evicted.
+     *)
+    Definition DirSoundS: Prop :=
+      (post#[implDirIdx].(fst) = msiS \/ post#[implDirIdx].(snd) = msiS) ->
+      post#[implStatusIdx] = msiS.
+
+    (* Why exclusiveness of the directory:
+     * It's simple. We need to know [P.st = C2.st = I] when [C1.st = M] and
+     * [C1] is lock-free. By the soundness of the directory, we can get
+     * [P.dir.C1 = M]. Then by this exclusiveness, we can get
+     * [P.st = P.dir.C2 = I].
+     *)
+    Definition DirExcl1: Prop :=
+      msiM <= post#[implDirIdx].(fst) ->
+      post#[implStatusIdx] = msiI /\ post#[implDirIdx].(snd) = msiI.
+
+    Definition DirExcl2: Prop :=
+      msiM <= post#[implDirIdx].(snd) ->
+      post#[implStatusIdx] = msiI /\ post#[implDirIdx].(fst) = msiI.
+
+    Definition DirCorrectM: Prop :=
+      msiM <= post#[implStatusIdx] ->
+      post#[implDirIdx].(fst) = msiI /\ post#[implDirIdx].(snd) = msiI.
+    
+    Definition DirCorrectS: Prop :=
+      post#[implStatusIdx] = msiS ->
+      (post#[implDirIdx].(fst) <= msiS /\ post#[implDirIdx].(snd) <= msiS).
+    
+    Definition DirInvP: Prop :=
+      DirSoundS /\ DirExcl1 /\ DirExcl2 /\
+      DirCorrectM /\ DirCorrectS.
+
+  End InvDir.
+
+  Section DownLockInv.
+    Variables (post: OState ImplOStateIfc)
+              (porq: ORq Msg).
+
+    Definition ParentDownRsS1 (rqid: RqInfo Msg): Prop :=
+      rqid.(rqi_msg).(msg_id) = msiDownRqS ->
+      msiM <= post#[implDirIdx].(snd).
+      
+    Definition ParentDownRsS2 (rqid: RqInfo Msg): Prop :=
+      rqid.(rqi_msg).(msg_id) = msiDownRqS ->
+      msiM <= post#[implDirIdx].(fst).
+
+    Definition ParentDownRsI1 (rqid: RqInfo Msg): Prop :=
+      rqid.(rqi_msg).(msg_id) = msiDownRqI ->
+      msiS <= post#[implDirIdx].(snd).
+
+    Definition ParentDownRsI2 (rqid: RqInfo Msg): Prop :=
+      rqid.(rqi_msg).(msg_id) = msiDownRqI ->
+      msiS <= post#[implDirIdx].(fst).
+
+    Definition ParentDownLockBack: Prop :=
+      rqid <+- porq@[downRq];
+        (rqid.(rqi_minds_rss) = [c1pRs] ->
+         rqid.(rqi_midx_rsb) = pc2 /\ ParentDownRsS2 rqid /\ ParentDownRsS2 rqid) /\
+        (rqid.(rqi_minds_rss) = [c2pRs] ->
+         rqid.(rqi_midx_rsb) = pc1 /\ ParentDownRsS1 rqid /\ ParentDownRsI1 rqid).
+
+    Definition DownLockInv: Prop :=
+      ParentDownLockBack.
+
+  End DownLockInv.
+
+  Definition ImplInvB (st: MState ImplOStateIfc): Prop :=
+    post <-- (bst_oss st)@[parentIdx];
+      porq <-- (bst_orqs st)@[parentIdx];
+      DirInvP post /\ DownLockInv post porq.
+
+  Hint Unfold DirSoundS DirExcl1 DirExcl2
+       DirCorrectM DirCorrectS DirInvP
+       ParentDownRsS1 ParentDownRsS2 ParentDownRsI1 ParentDownRsI2
+       ParentDownLockBack DownLockInv
+       ImplInvB: RuleConds.
+
+  Ltac disc_impl_inv_b :=
+    repeat
+      match goal with
+      | [H: getDir _ _ = _ |- _] => unfold getDir in H; simpl in H
+      | [H1: msg_id _ = _, H2: msg_id _ = _ |- _] => rewrite H1 in H2; discriminate
+      end.
+
+  Ltac disc_rule_custom ::=
+    try disc_impl_inv_b.
+
+  Lemma implInvB_init:
+    ImplInvB (initsOf impl).
+  Proof.
+    red; simpl.
+    unfold implOStatesInit, implORqsInit; mred.
+    simpl; repeat split;
+      try (simpl in *; solve_msi_false; fail); auto.
+  Qed.
+
+  Lemma implInvB_invStep:
+    InvStep impl step_m ImplInvB.
+  Proof.
+    unfold InvStep; intros.
+    inv H1; try assumption.
+    dest_in.
+
+    (* It roughly takes 2 minutes to solve all 40 cases. *)
+    all: solve_rule_conds_ex; solve_msi; fail.
+  Qed.
+
+End Inv.
+
+Hint Unfold DirSoundS DirExcl1 DirExcl2
+     DirCorrectM DirCorrectS DirInvP
+     ParentDownRsS1 ParentDownRsS2 ParentDownRsI1 ParentDownRsI2
+     ParentDownLockBack DownLockInv
+     ImplInvB: RuleConds.
+
+Close Scope list.
+Close Scope hvec.
+Close Scope fmap.
+
